Superposition_Calculus/Term_Ordering_Lifting.thy
@@ -1,39 +1,111 @@
 theory Term_Ordering_Lifting
-  imports Clausal_Calculus_Extra Min_Max_Least_Greatest_Multiset
+  imports 
+    Clausal_Calculus_Extra 
+    Min_Max_Least_Greatest_Multiset
+    Functional_Substitution_Lifting
+    Nonground_Clause
 begin
+
+locale relation_restriction = 
+  fixes R :: "'a \<Rightarrow> 'a \<Rightarrow> bool" and lift :: "'b \<Rightarrow> 'a" (* TODO: Name *)
+  assumes inj_lift [intro]: "inj lift"
+begin
+
+definition R\<^sub>r :: "'b \<Rightarrow> 'b \<Rightarrow> bool" where
+  "R\<^sub>r b b' \<equiv> R (lift b) (lift b')"
+
+end
 
 locale strict_order = 
   fixes
-    R :: "'a \<Rightarrow> 'a \<Rightarrow> bool" (infix "\<prec>" 50)
+    less :: "'a \<Rightarrow> 'a \<Rightarrow> bool" (infix "\<prec>" 50)
   assumes
     transp [intro]: "transp (\<prec>)" and
     asymp [intro]: "asymp (\<prec>)"
 begin
+
+abbreviation less_eq where "less_eq \<equiv> (\<prec>)\<^sup>=\<^sup>="
+
+notation less_eq (infix "\<preceq>" 50)
  
-sublocale order "(\<prec>)\<^sup>=\<^sup>=" "(\<prec>)"
+sublocale order "(\<preceq>)" "(\<prec>)"
   by(rule order_reflclp_if_transp_and_asymp[OF transp asymp])
 
 end
+
+(* TODO: name *)
+locale strict_order_restriction = strict_order + relation_restriction where R = "(\<prec>)"
+begin
+
+abbreviation "less\<^sub>r \<equiv> R\<^sub>r"
+
+notation less\<^sub>r (infix "\<prec>\<^sub>r" 50)
+
+(* TODO: Without name! *)
+sublocale restriction: strict_order "(\<prec>\<^sub>r)"
+  by unfold_locales (auto simp: R\<^sub>r_def transp_def)
+
+notation restriction.less_eq (infix "\<preceq>\<^sub>r" 50)
+
+end
+
+locale restricted_wellfounded_strict_order = strict_order +
+  fixes restriction
+  assumes wfp_on [intro]: "wfp_on restriction (\<prec>)"
 
 locale wellfounded_strict_order = strict_order +
   assumes wfp [intro]: "wfp (\<prec>)"
 begin
 
-lemma wfp_on [intro]: "\<And>X. wfp_on X (\<prec>)"
-  using wfp_on_subset by auto
+sublocale restricted_wellfounded_strict_order "(\<prec>)" UNIV
+  by unfold_locales (rule wfp)
 
 end
 
-locale total_on_strict_order = strict_order +
-  fixes X
-  assumes totalp_on [intro]: "totalp_on X (\<prec>)"
-
-locale total_strict_order = total_on_strict_order where X = UNIV
+locale wellfounded_strict_order_restriction = 
+  strict_order_restriction +
+  restricted_wellfounded_strict_order where restriction = "range lift" and less = "(\<prec>)"
 begin
 
-sublocale linorder "(\<prec>)\<^sup>=\<^sup>=" "(\<prec>)"
+sublocale restriction: wellfounded_strict_order "(\<prec>\<^sub>r)"
+proof unfold_locales
+  show "wfp (\<prec>\<^sub>r)"
+    using wfp_on_if_convertible_to_wfp_on[OF wfp_on]
+    unfolding R\<^sub>r_def
+    by simp
+qed
+
+end
+
+locale restricted_total_strict_order = strict_order +
+  fixes restriction
+  assumes totalp_on [intro]: "totalp_on restriction (\<prec>)"
+
+locale total_strict_order = strict_order +
+  assumes totalp [intro]: "totalp (\<prec>)"
+begin
+
+sublocale linorder "(\<preceq>)" "(\<prec>)"
   using totalpD
   by unfold_locales fastforce
+
+sublocale restricted_total_strict_order "(\<prec>)" UNIV
+  by unfold_locales (rule totalp)
+
+end
+
+locale total_strict_order_restriction = 
+  strict_order_restriction + 
+  restricted_total_strict_order where restriction = "range lift" and less = "(\<prec>)"
+begin
+
+sublocale restriction: total_strict_order "(\<prec>\<^sub>r)"
+proof unfold_locales
+  show "totalp (\<prec>\<^sub>r)"
+    using totalp_on inj_lift
+    unfolding R\<^sub>r_def totalp_on_def inj_def
+    by blast
+qed
 
 end
 
@@ -41,17 +113,19 @@ locale multiset_extension = base: strict_order +
   fixes to_mset :: "'b \<Rightarrow> 'a multiset"
 begin
 
-definition multiset_extension :: "'b \<Rightarrow> 'b \<Rightarrow> bool" (infix "\<prec>\<^sub>m" 50) where
+definition multiset_extension :: "'b \<Rightarrow> 'b \<Rightarrow> bool" where
   "multiset_extension b1 b2 \<equiv> multp (\<prec>) (to_mset b1) (to_mset b2)"
+
+notation multiset_extension (infix "\<prec>\<^sub>m" 50)
 
 sublocale strict_order "(\<prec>\<^sub>m)"
 proof unfold_locales
-  show "\<And>X. transp_on X (\<prec>\<^sub>m)"
+  show "transp (\<prec>\<^sub>m)"
     using transp_multp[OF base.transp]
     unfolding multiset_extension_def transp_on_def
     by blast
 next
-  show "\<And>X. asymp_on X (\<prec>\<^sub>m)"
+  show "asymp (\<prec>\<^sub>m)"
     unfolding multiset_extension_def
     by (simp add: asympD asymp_multp\<^sub>H\<^sub>O asymp_onI multp_eq_multp\<^sub>H\<^sub>O)
 qed
@@ -65,7 +139,7 @@ begin
 
 sublocale wellfounded_strict_order "(\<prec>\<^sub>m)"
 proof unfold_locales
-  show "\<And>X. wfp_on X (\<prec>\<^sub>m)"
+  show "wfp (\<prec>\<^sub>m)"
     unfolding multiset_extension_def
     using wfp_multp
     by (metis (no_types, lifting) base.wfp top_greatest wfp_if_convertible_to_wfp wfp_on_subset)
@@ -73,19 +147,18 @@ qed
 
 end
 
-
-locale total_on_multiset_extension = 
-  base: total_on_strict_order + multiset_extension +
-  assumes inj_on_to_mset: "inj_on to_mset {b. set_mset (to_mset b) \<subseteq> X}"
+locale restricted_total_multiset_extension = 
+  base: restricted_total_strict_order + multiset_extension +
+  assumes inj_on_to_mset: "inj_on to_mset {b. set_mset (to_mset b) \<subseteq> restriction}"
 begin
 
-sublocale total_on_strict_order "(\<prec>\<^sub>m)" "{b. set_mset (to_mset b) \<subseteq> X}"
+sublocale restricted_total_strict_order "(\<prec>\<^sub>m)" "{b. set_mset (to_mset b) \<subseteq> restriction}"
 proof unfold_locales
-  have "totalp_on {b. set_mset b \<subseteq> X} (multp (\<prec>))"
+  have "totalp_on {b. set_mset b \<subseteq> restriction} (multp (\<prec>))"
     using totalp_on_multp[OF base.totalp_on base.transp]
     by fastforce
 
-  then show "totalp_on {b. set_mset (to_mset b) \<subseteq> X} (\<prec>\<^sub>m)"
+  then show "totalp_on {b. set_mset (to_mset b) \<subseteq> restriction} (\<prec>\<^sub>m)"
     using inj_on_to_mset
     unfolding multiset_extension_def totalp_on_def inj_on_def
     by auto
@@ -93,7 +166,210 @@ qed
 
 end
 
-locale total_multiset_extension = total_on_multiset_extension where X = UNIV
+locale grounded_order = 
+  strict_order_restriction where lift = "from_ground :: 'expr\<^sub>G \<Rightarrow> 'expr" + 
+  grounding
+begin
+
+lemma to_ground_less\<^sub>r [simp]: 
+  assumes "is_ground e" and "is_ground e'"
+  shows "to_ground e \<prec>\<^sub>r to_ground e' \<longleftrightarrow> e \<prec> e'"
+  by (simp add: assms R\<^sub>r_def) (* TODO: Name R\<^sub>r_def *)
+
+lemma to_ground_less_eq\<^sub>r [simp]:
+  assumes "is_ground e" and "is_ground e'" 
+  shows "to_ground e \<preceq>\<^sub>r to_ground e' \<longleftrightarrow> e \<preceq> e'"
+  using assms obtain_grounding
+  by fastforce
+
+lemma less_eq\<^sub>r_from_ground [simp]:
+   "e\<^sub>G \<preceq>\<^sub>r e\<^sub>G' \<longleftrightarrow> from_ground e\<^sub>G \<preceq> from_ground e\<^sub>G'"
+  unfolding R\<^sub>r_def
+  by (simp add: inj_eq inj_lift)
+  
+end
+
+locale ground_subst_stable_grounded_order = grounded_order + 
+  assumes 
+    less_ground_subst_stability: 
+      "\<And>e\<^sub>1 e\<^sub>2 \<gamma>.
+        is_ground (e\<^sub>1 \<cdot> \<gamma>) \<Longrightarrow>
+        is_ground (e\<^sub>2 \<cdot> \<gamma>) \<Longrightarrow>
+        e\<^sub>1 \<prec> e\<^sub>2 \<Longrightarrow>
+        e\<^sub>1 \<cdot> \<gamma> \<prec> e\<^sub>2 \<cdot> \<gamma>"
+begin
+
+(* TODO: Names *)
+lemma less_eq_ground_subst_stability:
+  assumes "is_ground (term\<^sub>1 \<cdot> \<gamma>)" "is_ground (term\<^sub>2 \<cdot> \<gamma>)"  "term\<^sub>1 \<preceq> term\<^sub>2"
+  shows "term\<^sub>1 \<cdot> \<gamma> \<preceq> term\<^sub>2 \<cdot> \<gamma>"
+  using less_ground_subst_stability[OF assms(1, 2)] assms(3)
+  by auto
+
+lemma less\<^sub>t_less_eq\<^sub>t_ground_subst_stability:
+  assumes 
+    "is_ground (term\<^sub>1 \<cdot> \<gamma>)"
+    "is_ground (term\<^sub>2 \<cdot> \<gamma>)"
+    "term\<^sub>1 \<cdot> \<gamma> \<prec> term\<^sub>2 \<cdot> \<gamma>"
+  shows
+    "\<not> term\<^sub>2 \<preceq> term\<^sub>1"
+proof
+  assume assumption: "term\<^sub>2 \<preceq> term\<^sub>1"
+
+  have "term\<^sub>2 \<cdot> \<gamma> \<preceq> term\<^sub>1 \<cdot> \<gamma>"
+    using less_eq_ground_subst_stability[OF 
+            assms(2, 1)
+            assumption
+           ].
+
+  then show False 
+    using assms(3) by order
+qed
+
+
+end
+
+
+locale less_subst_upd_grounded_order =
+  fixes base_less less base_is_ground is_ground subst vars
+  assumes
+    less_subst_upd:
+    "\<And>update x \<gamma> expr. 
+      base_is_ground update \<Longrightarrow>
+      base_less update (\<gamma> x) \<Longrightarrow> 
+      is_ground (subst expr \<gamma>) \<Longrightarrow>
+      x \<in> vars expr \<Longrightarrow>
+      less (subst expr (\<gamma>(x := update))) (subst expr \<gamma>)"
+
+(* TODO: Name *)
+locale grounded_total_strict_order = 
+  total_strict_order_restriction where lift = "from_ground :: 'expr\<^sub>G \<Rightarrow> 'expr" +
+  grounded_order
+begin
+
+lemma not_less_eq [simp]: 
+  assumes "is_ground e" and "is_ground e'"
+  shows "\<not> e' \<preceq> e \<longleftrightarrow> e \<prec> e'"
+  using assms totalp_on
+  unfolding totalp_on_def is_ground_iff_range_from_ground
+  by auto
+  
+end
+
+locale multiset_extension_restriction = 
+  sub: strict_order_restriction where lift = "sub_from_ground :: 'sub\<^sub>G \<Rightarrow> 'sub" + 
+  multiset_extension where to_mset = to_mset +
+  grounding_lifting where id_subst = id_subst and to_set = to_set and to_set_ground = to_set_ground
+for 
+  to_mset :: "'expr \<Rightarrow> 'sub multiset" and 
+  id_subst :: "'var \<Rightarrow> 'base" and
+  to_set :: "'expr \<Rightarrow> 'sub set" and
+  to_set_ground :: "'expr\<^sub>G \<Rightarrow> 'sub\<^sub>G set" +
+assumes 
+  to_mset_to_set: "\<And>expr. set_mset (to_mset expr) = to_set expr" and
+  inj_to_mset: "inj to_mset" (* TODO: *)
+begin
+
+sublocale strict_order_restriction "(\<prec>\<^sub>m)" from_ground
+  by(unfold_locales)(rule inj_from_ground)
+
+end
+
+(* TODO: Name *)
+locale total_multiset_extension_restriction = 
+  multiset_extension_restriction +
+  sub: total_strict_order_restriction where lift = "sub_from_ground"
+begin
+
+sublocale total_strict_order_restriction "(\<prec>\<^sub>m)" from_ground
+proof unfold_locales
+  have "totalp_on {expr. set_mset expr \<subseteq> range sub_from_ground} (multp (\<prec>))"
+    using sub.totalp_on totalp_on_multp by fastforce
+
+  then have "totalp_on {expr. set_mset (to_mset expr) \<subseteq> range sub_from_ground} (\<prec>\<^sub>m)"
+    using inj_to_mset
+    unfolding inj_def multiset_extension_def totalp_on_def
+    by blast
+
+  then show "totalp_on (range from_ground) (\<prec>\<^sub>m)"
+    unfolding multiset_extension_def totalp_on_def from_ground_def
+    by (simp add: image_mono to_mset_to_set)
+qed
+  
+end
+
+locale based_multiset_extension_restriction = 
+  based_functional_substitution_lifting where base_vars = base_vars +
+  multiset_extension_restriction +
+  sub: strict_order +
+  base: strict_order where less = base_less 
+for base_vars :: "'base \<Rightarrow> 'var set" and base_less :: "'base \<Rightarrow> 'base \<Rightarrow> bool"
+ 
+
+(* TODO: Name + totality not needed! *)
+locale total_multiset_extension_restriction_stable = 
+  multiset_extension_restriction + 
+  sub: ground_subst_stable_grounded_order where 
+  less = less and subst = sub_subst and vars = sub_vars and from_ground = sub_from_ground and 
+  to_ground = sub_to_ground +
+assumes to_mset_map: "\<And>f b. to_mset (map f b) = image_mset f (to_mset b)"
+begin
+
+sublocale ground_subst_stable_grounded_order where 
+  less = "(\<prec>\<^sub>m)" and subst = subst and vars = vars and from_ground = from_ground and 
+  to_ground = to_ground
+proof unfold_locales
+
+  fix e\<^sub>1 e\<^sub>2 \<gamma> 
+  assume "is_ground (e\<^sub>1 \<cdot> \<gamma>)" "is_ground (e\<^sub>2 \<cdot> \<gamma>)" and a: "e\<^sub>1 \<prec>\<^sub>m e\<^sub>2" 
+
+  moreover then have "monotone_on (set_mset (to_mset e\<^sub>1 + to_mset e\<^sub>2)) (\<prec>) (\<prec>) (\<lambda>sub. sub \<cdot>\<^sub>s \<gamma>)"
+    using monotone_onI sub.less_ground_subst_stability
+    by (smt (verit, best) to_mset_to_set to_set_is_ground_subst union_iff)
+  
+  then show "e\<^sub>1 \<cdot> \<gamma> \<prec>\<^sub>m e\<^sub>2 \<cdot> \<gamma>"
+    unfolding multiset_extension_def subst_def to_mset_map
+    by(rule multp_map_strong[OF sub.transp _ a[unfolded multiset_extension_def]])
+qed
+
+end
+
+
+locale multiset_extension_restriction_upd = 
+  based_multiset_extension_restriction +
+  sub: less_subst_upd_grounded_order where 
+  less = less and base_is_ground = base.is_ground and is_ground = sub.is_ground
+  and vars = sub_vars and subst = sub_subst +
+  assumes to_mset_map: "\<And>f b. to_mset (map f b) = image_mset f (to_mset b)"
+begin 
+
+
+sublocale less_subst_upd_grounded_order where 
+  less = "(\<prec>\<^sub>m)" and base_is_ground = base.is_ground and is_ground = is_ground
+  and vars = vars and subst = subst 
+proof unfold_locales
+  fix update x \<gamma> expr
+  assume assms: 
+    "base.is_ground update" "base_less update (\<gamma> x)" "is_ground (expr \<cdot> \<gamma>)" "x \<in> vars expr"
+
+  moreover then have "\<forall>sub \<in># to_mset expr. sub.less_eq (sub \<cdot>\<^sub>s \<gamma>(x := update)) (sub \<cdot>\<^sub>s \<gamma>)" (* TODO: sub.less_eq *)
+    using sub.less_subst_upd sub.subst_reduntant_upd
+    by (metis sub.order.refl sub.order.strict_iff_not to_mset_to_set to_set_is_ground_subst)
+
+  moreover have "\<exists>sub \<in># to_mset expr. sub \<cdot>\<^sub>s \<gamma>(x := update) \<prec> (sub \<cdot>\<^sub>s \<gamma>)"
+    using sub.less_subst_upd assms
+    unfolding vars_def subst_def to_mset_to_set
+    by fastforce
+
+  ultimately show "expr \<cdot> \<gamma>(x := update) \<prec>\<^sub>m expr \<cdot> \<gamma> "
+    unfolding multiset_extension_def subst_def to_mset_map
+    using multp_all_lesseq_ex_less[OF sub.asymp sub.transp]
+    by meson
+qed
+
+end
+
+locale total_multiset_extension = restricted_total_multiset_extension where restriction = UNIV
 begin
 
 lemma inj_to_mset: "inj to_mset"
@@ -108,156 +384,187 @@ sublocale total_strict_order "(\<prec>\<^sub>m)"
 
 end
 
-locale restricted_term_ordering_lifting =
-  fixes
-    less\<^sub>t :: "'t \<Rightarrow> 't \<Rightarrow> bool" (infix "\<prec>\<^sub>t" 50) and
-    X :: "'t set"
-  assumes
-    less\<^sub>t_transp [intro]: "transp (\<prec>\<^sub>t)" and
-    less\<^sub>t_asymp [intro]: "asymp (\<prec>\<^sub>t)" and
-    less\<^sub>t_wfp_on [intro]: "wfp_on X (\<prec>\<^sub>t)" and
-    less\<^sub>t_totalp_on [intro]: "totalp_on X (\<prec>\<^sub>t)" 
+locale total_wellfounded_multiset_extension = 
+  wellfounded_multiset_extension + total_multiset_extension
+
+(* TODO: Name*)
+locale literal_order = strict_order where less = less for 
+  less :: "'t uprod literal \<Rightarrow> 't uprod literal \<Rightarrow> bool"
 begin
 
-abbreviation less_eq\<^sub>t where
-  "less_eq\<^sub>t \<equiv> (\<prec>\<^sub>t)\<^sup>=\<^sup>="
-
-notation less_eq\<^sub>t (infix "\<preceq>\<^sub>t" 50)
-
-sublocale term_order: total_on_strict_order "(\<prec>\<^sub>t)"
-  by unfold_locales auto
-
-abbreviation literal_order_restriction where 
-  "literal_order_restriction \<equiv> {b. set_mset (mset_lit b) \<subseteq> X}"
-
-sublocale literal_order: total_on_multiset_extension where R = "(\<prec>\<^sub>t)" and to_mset = mset_lit 
-  using inj_mset_lit
-  by unfold_locales (auto simp: inj_on_def)
-
-abbreviation less\<^sub>l where
-  "less\<^sub>l \<equiv> literal_order.multiset_extension"
-
-notation less\<^sub>l (infix "\<prec>\<^sub>l" 50) 
-
-abbreviation less_eq\<^sub>l where
-  "less_eq\<^sub>l \<equiv> (\<prec>\<^sub>l)\<^sup>=\<^sup>="
-
-notation less_eq\<^sub>l (infix "\<preceq>\<^sub>l" 50)
-
-lemmas less\<^sub>l_def = literal_order.multiset_extension_def
-
-sublocale clause_order: total_on_multiset_extension where 
-  R = "(\<prec>\<^sub>l)" and to_mset = "\<lambda>x. x" and X = literal_order_restriction
-  by unfold_locales simp
-
-abbreviation less\<^sub>c where
-  "less\<^sub>c \<equiv> clause_order.multiset_extension"
-
-notation less\<^sub>c (infix "\<prec>\<^sub>c" 50) 
-
-abbreviation less_eq\<^sub>c where
-  "less_eq\<^sub>c \<equiv> (\<prec>\<^sub>c)\<^sup>=\<^sup>="
-
-notation less_eq\<^sub>c (infix "\<preceq>\<^sub>c" 50)
-
-lemmas less\<^sub>c_def = clause_order.multiset_extension_def
-
 abbreviation is_maximal\<^sub>l :: "'t uprod literal \<Rightarrow> 't uprod clause \<Rightarrow> bool" where
-  "is_maximal\<^sub>l L M \<equiv> is_maximal_in_mset_wrt (\<prec>\<^sub>l) M L"
+  "is_maximal\<^sub>l L M \<equiv> is_maximal_in_mset_wrt less M L"
 
 abbreviation is_strictly_maximal\<^sub>l :: "'t uprod literal \<Rightarrow> 't uprod clause \<Rightarrow> bool" where
-  "is_strictly_maximal\<^sub>l L M \<equiv> is_strictly_maximal_in_mset_wrt (\<prec>\<^sub>l) M L"
+  "is_strictly_maximal\<^sub>l L M \<equiv> is_strictly_maximal_in_mset_wrt less M L"
 
-lemmas is_maximal\<^sub>l_def = literal_order.is_maximal_in_mset_iff
+lemmas is_maximal\<^sub>l_def = is_maximal_in_mset_iff
 
-lemmas is_strictly_maximal\<^sub>l_def = literal_order.is_strictly_maximal_in_mset_iff
+lemmas is_strictly_maximal\<^sub>l_def = is_strictly_maximal_in_mset_iff
 
-lemmas is_maximal\<^sub>l_if_is_strictly_maximal\<^sub>l = 
-  literal_order.is_maximal_in_mset_if_is_strictly_maximal_in_mset
+lemmas is_maximal\<^sub>l_if_is_strictly_maximal\<^sub>l = is_maximal_in_mset_if_is_strictly_maximal_in_mset
 
 lemma maximal\<^sub>l_in_clause:
-  assumes "is_maximal\<^sub>l literal clause"
-  shows "literal \<in># clause"
+  assumes "is_maximal\<^sub>l l C"
+  shows "l \<in># C"
   using assms 
   unfolding is_maximal\<^sub>l_def
   by(rule conjunct1)
 
 lemma strictly_maximal\<^sub>l_in_clause:
-  assumes "is_strictly_maximal\<^sub>l literal clause"
-  shows "literal \<in># clause"
+  assumes "is_strictly_maximal\<^sub>l l C"
+  shows "l \<in># C"
   using assms  
   unfolding is_strictly_maximal\<^sub>l_def
   by(rule conjunct1)
 
-lemma is_maximal\<^sub>l_empty [simp]: 
-  assumes "is_maximal\<^sub>l literal {#}"  
-  shows False
-  using assms maximal\<^sub>l_in_clause
+lemma is_maximal\<^sub>l_empty [simp]: "\<not>is_maximal\<^sub>l l {#}"  
+  using maximal\<^sub>l_in_clause
   by fastforce
 
-lemma is_strictly_maximal\<^sub>l_empty [simp]: 
-  assumes "is_strictly_maximal\<^sub>l literal {#}"  
-  shows False
-  using assms strictly_maximal\<^sub>l_in_clause
+lemma is_strictly_maximal\<^sub>l_empty [simp]: "\<not>is_strictly_maximal\<^sub>l l {#}"
+  using strictly_maximal\<^sub>l_in_clause
   by fastforce
 
 end
 
-locale total_wellfounded_multiset_extension = 
-  wellfounded_multiset_extension + total_multiset_extension
-
-locale term_ordering_lifting = restricted_term_ordering_lifting where X = UNIV
+locale restricted_term_ordering_lifting =
+  term_order: restricted_total_strict_order where less = "(\<prec>\<^sub>t)" +
+  term_order: restricted_wellfounded_strict_order where less = "(\<prec>\<^sub>t)"
+  for
+    less\<^sub>t :: "'t \<Rightarrow> 't \<Rightarrow> bool" (infix "\<prec>\<^sub>t" 50) 
 begin
 
-sublocale term_order: wellfounded_strict_order "(\<prec>\<^sub>t)"
-  using wfp_on_subset
+notation term_order.less_eq (infix "\<preceq>\<^sub>t" 50)
+
+abbreviation literal_order_restriction where 
+  "literal_order_restriction \<equiv> {b. set_mset (mset_lit b) \<subseteq> restriction}"
+
+sublocale literal_order: restricted_total_multiset_extension where 
+  less = "(\<prec>\<^sub>t)" and to_mset = mset_lit
+  using inj_mset_lit
+  by unfold_locales (auto simp: inj_on_def)
+
+notation literal_order.multiset_extension (infix "\<prec>\<^sub>l" 50)
+notation literal_order.less_eq (infix "\<preceq>\<^sub>l" 50)
+
+lemmas less\<^sub>l_def = literal_order.multiset_extension_def
+
+sublocale clause_order: restricted_total_multiset_extension where 
+  less = "(\<prec>\<^sub>l)" and to_mset = "\<lambda>x. x" and restriction = literal_order_restriction
   by unfold_locales auto
 
-sublocale term_order: total_strict_order "(\<prec>\<^sub>t)"
+notation clause_order.multiset_extension (infix "\<prec>\<^sub>c" 50) 
+notation clause_order.less_eq (infix "\<preceq>\<^sub>c" 50)
+
+lemmas less\<^sub>c_def = clause_order.multiset_extension_def
+
+sublocale literal_order "(\<prec>\<^sub>l)"
   by unfold_locales
 
-sublocale literal_order: wellfounded_multiset_extension where R = "(\<prec>\<^sub>t)" and to_mset = mset_lit
+end
+
+locale grounded_term_ordering_lifting =
+  restricted_term_ordering_lifting where restriction = "range term.from_ground"
+begin
+
+sublocale term_order: 
+  total_strict_order_restriction where less = less\<^sub>t and lift = term.from_ground
+  apply unfold_locales
+  by (simp add: inj_term_of_gterm)
+
+sublocale term_order: grounded_total_strict_order where 
+  less = less\<^sub>t and from_ground = term.from_ground and comp_subst = "(\<odot>)" and subst = "(\<cdot>t)" and
+  vars = term.vars and id_subst = Var and to_ground = term.to_ground
   by unfold_locales
 
-sublocale literal_order: total_multiset_extension where R = "(\<prec>\<^sub>t)" and to_mset = mset_lit
+(* TODO *)
+notation term_order.R\<^sub>r (infix "\<prec>\<^sub>t\<^sub>G" 50)
+notation term_order.restriction.less_eq (infix "\<preceq>\<^sub>t\<^sub>G" 50)
+lemmas less\<^sub>t\<^sub>G_def = term_order.R\<^sub>r_def
+
+(* TODO: Duplication *)
+sublocale literal_order: total_multiset_extension_restriction where 
+  less = "(\<prec>\<^sub>t)" and comp_subst = "(\<odot>)" and sub_to_ground = term.to_ground and 
+  sub_from_ground = term.from_ground and sub_vars = term.vars and sub_subst = "(\<cdot>t)" and 
+  map = map_literal_term and to_ground_map = map_literal_term and 
+  from_ground_map = map_literal_term and ground_map = map_literal_term and to_mset = mset_lit and 
+  id_subst = Var and to_set = literal_to_term_set and to_set_ground = literal_to_term_set
+  using inj_mset_lit term.inj_from_ground
+  by unfold_locales auto
+
+(* TODO! \<longrightarrow> Same for clause
+sublocale literal_order: grounded_total_strict_order where 
+  less = "(\<prec>\<^sub>l)" and from_ground = literal.from_ground and comp_subst = "(\<odot>)" and subst = "(\<cdot>l)" and
+  vars = literal.vars and id_subst = Var and to_ground = literal.to_ground
+  by unfold_locales*)
+
+notation literal_order.R\<^sub>r (infix "\<prec>\<^sub>l\<^sub>G" 50)
+notation literal_order.restriction.less_eq (infix "\<preceq>\<^sub>l\<^sub>G" 50)
+
+lemmas less\<^sub>l\<^sub>G_def = literal_order.R\<^sub>r_def
+
+
+sublocale clause: total_multiset_extension_restriction where 
+  less = "(\<prec>\<^sub>l)" and to_mset = "\<lambda>x. x" and comp_subst = "(\<odot>)" and sub_to_ground = literal'.to_ground and 
+  sub_from_ground = literal'.from_ground and sub_vars = literal'.vars and sub_subst = "(\<cdot>l)" and 
+  map = image_mset and to_ground_map = image_mset and 
+  from_ground_map = image_mset and ground_map = image_mset and 
+  id_subst = Var and to_set = set_mset and to_set_ground = set_mset
+  by unfold_locales auto
+
+notation clause.R\<^sub>r (infix "\<prec>\<^sub>c\<^sub>G" 50)
+notation clause.restriction.less_eq (infix "\<preceq>\<^sub>c\<^sub>G" 50)
+
+lemmas less\<^sub>c\<^sub>G_def = clause.R\<^sub>r_def
+
+sublocale restriction: literal_order "(\<prec>\<^sub>l\<^sub>G)"
   by unfold_locales
 
-sublocale clause_order: wellfounded_multiset_extension where R = "(\<prec>\<^sub>l)"  and to_mset = "\<lambda>x. x" 
+(* TODO!!  *)
+lemma ground_is_maximal\<^sub>l_iff_is_maximal\<^sub>l: 
+  "restriction.is_maximal\<^sub>l l\<^sub>G C\<^sub>G \<longleftrightarrow> is_maximal\<^sub>l (literal.from_ground l\<^sub>G) (clause.from_ground C\<^sub>G)"
+   unfolding 
+    is_maximal\<^sub>l_def
+    restriction.is_maximal\<^sub>l_def
+    clause.ground_sub_in_ground[symmetric]
+   by (smt (verit, best) atom.from_ground_def image_iff less\<^sub>l\<^sub>G_def literal'.from_ground_def literal.from_ground_def literal.map_cong0 literal_order.dual_order.strict_iff_order clause.ground_sub_in_ground clause.to_set_from_ground)
+   
+lemma ground_is_strictly_maximal\<^sub>l_iff_is_strictly_maximal\<^sub>l:
+  "restriction.is_strictly_maximal\<^sub>l l\<^sub>G C\<^sub>G \<longleftrightarrow> 
+    is_strictly_maximal\<^sub>l (literal.from_ground l\<^sub>G) (clause.from_ground C\<^sub>G)"
+  unfolding 
+    restriction.is_strictly_maximal\<^sub>l_def
+    is_strictly_maximal\<^sub>l_def
+    clause.ground_sub_in_ground[symmetric]
+    remove1_mset_literal_from_ground
+    clause.ground_sub
+  apply auto
+  apply (metis (mono_tags, lifting) atom.from_ground_def image_iff literal'.from_ground_def literal.from_ground_def literal.map_cong0 local.clause.to_set_from_ground)
+  apply (smt (verit, best) Nonground_Clause.clause.from_ground_def atom.from_ground_def image_iff image_mset_cong2 less\<^sub>l\<^sub>G_def literal'.from_ground_def literal.from_ground_def literal.map_cong0 local.clause.from_ground_def local.clause.to_set_from_ground remove1_mset_literal_from_ground)
+  apply (metis Nonground_Clause.clause.from_ground_def Nonground_Clause.clause.ground_sub_in_ground atom.from_ground_def image_mset_cong2 literal'.from_ground_def literal.from_ground_def literal.map_cong0 local.clause.from_ground_def remove1_mset_literal_from_ground)
+  apply (metis atom.from_ground_def literal'.from_ground_def literal.from_ground_def literal.map_cong0 local.clause.ground_sub_in_ground)
+  apply (metis (mono_tags, lifting) Nonground_Clause.clause.from_ground_def Nonground_Clause.clause.ground_sub_in_ground atom.from_ground_def image_mset_cong2 less\<^sub>l\<^sub>G_def literal'.from_ground_def literal.from_ground_def literal.map_cong0 local.clause.from_ground_def remove1_mset_literal_from_ground)
+  by (metis (mono_tags, lifting) Nonground_Clause.clause.from_ground_def Nonground_Clause.clause.to_set_from_ground atom.from_ground_def image_iff image_mset_cong2 literal'.from_ground_def literal.from_ground_def literal.map_cong0 local.clause.from_ground_def remove1_mset_literal_from_ground)
+ 
+end
+
+
+locale term_ordering_lifting =  
+  restricted_term_ordering_lifting where restriction = UNIV +
+  term_order: wellfounded_strict_order "(\<prec>\<^sub>t)" + 
+  term_order: total_strict_order "(\<prec>\<^sub>t)"
+begin
+
+sublocale literal_order: total_wellfounded_multiset_extension where 
+  less = "(\<prec>\<^sub>t)" and to_mset = mset_lit
   by unfold_locales
 
-sublocale clause_order: total_multiset_extension where R = "(\<prec>\<^sub>l)" and to_mset = "\<lambda>x. x"
+sublocale clause_order: total_wellfounded_multiset_extension where 
+  less = "(\<prec>\<^sub>l)"  and to_mset = "\<lambda>x. x" 
   by unfold_locales simp
 
 end
 
-locale grounded_term_ordering_lifting = restricted_term_ordering_lifting 
-  where X = "range from_ground" for from_ground :: "'g \<Rightarrow> 't" +
-  assumes
-    inj_from_ground: "inj from_ground" 
-begin
-
-definition less\<^sub>t\<^sub>G :: "'g \<Rightarrow> 'g \<Rightarrow> bool" (infix "\<prec>\<^sub>t\<^sub>G" 50) where
-  "term\<^sub>G\<^sub>1 \<prec>\<^sub>t\<^sub>G term\<^sub>G\<^sub>2 \<equiv> from_ground term\<^sub>G\<^sub>1 \<prec>\<^sub>t from_ground term\<^sub>G\<^sub>2"
-
-sublocale ground: term_ordering_lifting "(\<prec>\<^sub>t\<^sub>G)"
-proof unfold_locales
-  show "transp (\<prec>\<^sub>t\<^sub>G)"
-    unfolding less\<^sub>t\<^sub>G_def
-    using term_order.dual_order.strict_trans transp_def by blast
-next
-  show "asymp (\<prec>\<^sub>t\<^sub>G)"
-    unfolding less\<^sub>t\<^sub>G_def
-    by (simp add: asympI)
-next
-  show "wfp (\<prec>\<^sub>t\<^sub>G)"
-    unfolding less\<^sub>t\<^sub>G_def
-    by (metis less\<^sub>t_wfp_on wfp_on_image)
-next
-  show "totalp (\<prec>\<^sub>t\<^sub>G)"
-    unfolding less\<^sub>t\<^sub>G_def
-    using inj_from_ground totalp_on_image by blast
-qed
-
-end
 
 end
