Superposition_Calculus/Ground_Ordering.thy
@@ -12,65 +12,69 @@ locale ground_ordering = term_ordering_lifting "(\<prec>\<^sub>t)"
   for
     less\<^sub>t :: "'f gterm \<Rightarrow> 'f gterm \<Rightarrow> bool" (infix "\<prec>\<^sub>t" 50) +
   assumes
-    less\<^sub>t_compatible_with_gctxt[simp]: "\<And>c t t'. t \<prec>\<^sub>t t' \<Longrightarrow> c\<langle>t\<rangle>\<^sub>G \<prec>\<^sub>t c\<langle>t'\<rangle>\<^sub>G" and
+    less\<^sub>t_compatible_with_context [simp]: "\<And>c t t'. t \<prec>\<^sub>t t' \<Longrightarrow> c\<langle>t\<rangle>\<^sub>G \<prec>\<^sub>t c\<langle>t'\<rangle>\<^sub>G" and
     less\<^sub>t_if_subterm[simp]: "\<And>t c. c \<noteq> \<box> \<Longrightarrow> t \<prec>\<^sub>t c\<langle>t\<rangle>\<^sub>G"
 begin
 
-(*notation less\<^sub>c (infix "\<prec>\<^sub>c" 50) *)
-
-
-
-(* TODO: Names *)
-lemma lesseq_trm_if_subterm: "t \<preceq>\<^sub>t ctxt\<langle>t\<rangle>\<^sub>G"
+lemma less_eq\<^sub>t_if_subterm: "t \<preceq>\<^sub>t c\<langle>t\<rangle>\<^sub>G"
   using less\<^sub>t_if_subterm
   by (metis gctxt_ident_iff_eq_GHole reflclp_iff)
 
-lemma less\<^sub>t_compatible_with_gctxt':
-  assumes "ctxt\<langle>t\<rangle>\<^sub>G \<prec>\<^sub>t ctxt\<langle>t'\<rangle>\<^sub>G"
-  shows "t \<prec>\<^sub>t t'"
-proof(rule ccontr)
-  assume "\<not> t \<prec>\<^sub>t t'"
-  hence "t' \<preceq>\<^sub>t t"
-    by order
+lemma less\<^sub>t_compatible_with_context_iff: "c\<langle>t\<rangle>\<^sub>G \<prec>\<^sub>t c\<langle>t'\<rangle>\<^sub>G \<longleftrightarrow> t \<prec>\<^sub>t t'"
+proof(intro iffI)
+  assume less\<^sub>t_with_context: "c\<langle>t\<rangle>\<^sub>G \<prec>\<^sub>t c\<langle>t'\<rangle>\<^sub>G"
 
-  show False
-  proof(cases "t' = t")
-    case True
-    then have "ctxt\<langle>t\<rangle>\<^sub>G = ctxt\<langle>t'\<rangle>\<^sub>G"
-      by blast
-    then show False
-      using assms by order
-  next
-    case False
-    then have "t' \<prec>\<^sub>t t"
-      using \<open>t' \<preceq>\<^sub>t t\<close> by order
+  show "t \<prec>\<^sub>t t'"
+  proof(rule ccontr)
+    assume "\<not> t \<prec>\<^sub>t t'"
+    hence "t' \<preceq>\<^sub>t t"
+      by order
 
-    then have "ctxt\<langle>t'\<rangle>\<^sub>G \<prec>\<^sub>t ctxt\<langle>t\<rangle>\<^sub>G"
-      using less\<^sub>t_compatible_with_gctxt by metis
-      
-    then show ?thesis
-      using assms by order
+    show False
+    proof(cases "t' = t")
+      case True
+
+      then have "c\<langle>t\<rangle>\<^sub>G = c\<langle>t'\<rangle>\<^sub>G"
+        by blast
+
+      then show False
+        using less\<^sub>t_with_context 
+        by order
+    next
+      case False
+
+      then have "t' \<prec>\<^sub>t t"
+        using \<open>t' \<preceq>\<^sub>t t\<close> 
+        by order
+
+      then have "c\<langle>t'\<rangle>\<^sub>G \<prec>\<^sub>t c\<langle>t\<rangle>\<^sub>G"
+        using less\<^sub>t_compatible_with_context 
+        by metis
+
+      then show ?thesis
+        using less\<^sub>t_with_context 
+        by order
+    qed
   qed
+next
+  show "t \<prec>\<^sub>t t' \<Longrightarrow> c\<langle>t\<rangle>\<^sub>G \<prec>\<^sub>t c\<langle>t'\<rangle>\<^sub>G"
+    using less\<^sub>t_compatible_with_context.
 qed
-
-lemma less\<^sub>t_compatible_with_gctxt_iff: "ctxt\<langle>t\<rangle>\<^sub>G \<prec>\<^sub>t ctxt\<langle>t'\<rangle>\<^sub>G \<longleftrightarrow> t \<prec>\<^sub>t t'"
-  using less\<^sub>t_compatible_with_gctxt less\<^sub>t_compatible_with_gctxt' 
-  by blast
 
 lemma context_less_term_lesseq:
   assumes 
-    "\<And>t. ctxt\<langle>t\<rangle>\<^sub>G \<prec>\<^sub>t ctxt'\<langle>t\<rangle>\<^sub>G"
+    "\<And>t. c\<langle>t\<rangle>\<^sub>G \<prec>\<^sub>t c'\<langle>t\<rangle>\<^sub>G"
     "t \<preceq>\<^sub>t t'"
-  shows "ctxt\<langle>t\<rangle>\<^sub>G \<prec>\<^sub>t ctxt'\<langle>t'\<rangle>\<^sub>G"
-  using assms less\<^sub>t_compatible_with_gctxt
+  shows "c\<langle>t\<rangle>\<^sub>G \<prec>\<^sub>t c'\<langle>t'\<rangle>\<^sub>G"
+  using assms less\<^sub>t_compatible_with_context
   by (metis reflclp_iff term_order.dual_order.strict_trans)
 
 lemma context_lesseq_term_less:
   assumes 
-    "\<And>t. ctxt\<langle>t\<rangle>\<^sub>G \<preceq>\<^sub>t ctxt'\<langle>t\<rangle>\<^sub>G"
+    "\<And>t. c\<langle>t\<rangle>\<^sub>G \<preceq>\<^sub>t c'\<langle>t\<rangle>\<^sub>G"
     "t \<prec>\<^sub>t t'"
-  shows "ctxt\<langle>t\<rangle>\<^sub>G \<prec>\<^sub>t ctxt'\<langle>t'\<rangle>\<^sub>G"
-  using assms less\<^sub>t_compatible_with_gctxt term_order.dual_order.strict_trans1 
+  shows "c\<langle>t\<rangle>\<^sub>G \<prec>\<^sub>t c'\<langle>t'\<rangle>\<^sub>G"
+  using assms less\<^sub>t_compatible_with_context term_order.dual_order.strict_trans1 
   by blast
 
 end
